passes resolvekinds infertype inferwidth

src/HiEnv.v
@@ -11,9 +11,12 @@ Import Prenex Implicits.
 
 
 
-(****** Bundle type ******)
+(****** Aggregate type ******)
 
+Section Ftype.
 
+(* Variable var : eqType. *)
+  
 Inductive fflip : Type := Flipped | Nflip.
 
 Inductive ftype : Type :=
@@ -62,8 +65,8 @@ with ffield_eqn (f1 f2 : ffield) : bool :=
        | Fnil, Fnil => true
        | Fflips _ Nflip t1 fs1, Fflips _ Nflip t2 fs2
          => ftype_eqn t1 t2 && ffield_eqn fs1 fs2
-       | Fflips _ Flipped t1 fs1, Fflips _ Flipped t2 fs2
-         => ftype_eqn t1 t2 && ffield_eqn fs1 fs2
+       | Fflips v1 Flipped t1 fs1, Fflips v2 Flipped t2 fs2
+         => (v1 == v2) && ftype_eqn t1 t2 && ffield_eqn fs1 fs2
        | _, _ => false
        end.
 
@@ -114,6 +117,8 @@ Definition ffield_eqMixin := EqMixin ffield_eqP.
 Canonical ftype_eqType := Eval hnf in EqType ftype ftype_eqMixin.
 Canonical ffield_eqType := Eval hnf in EqType ffield ffield_eqMixin.
 
+End Ftype.
+
 Inductive fcomponent : Set :=
 | In_port
 | Instanceof
@@ -122,17 +127,9 @@ Inductive fcomponent : Set :=
 | Out_port
 | Register
 | Wire
+(* | Fmodule *)
 .
 
-(* Inductive fcomponent : Set := *)
-(* | In_port : ftype -> fcomponent *)
-(* | Instanceof : ftype -> fcomponent *)
-(* | Memory : ftype -> fcomponent *)
-(* | Node : ftype -> fcomponent *)
-(* | Out_port : ftype -> fcomponent *)
-(* | Register : ftype -> fcomponent *)
-(* | Wire : ftype -> fcomponent *)
-(* . *)
 
 (** eq dec *)
 Axiom component_eq_dec : forall {x y : fcomponent}, {x = y} + {x <> y}.
@@ -141,115 +138,6 @@ Axiom component_eqP : Equality.axiom component_eqn.
 Canonical component_eqMixin := EqMixin component_eqP.
 Canonical component_eqType := Eval hnf in EqType fcomponent component_eqMixin.
 
-(* A mapping from a variable to its component type *)
 
-Module Type CmpntEnv <: SsrFMap.
-
-  Include SsrFMap.
-
-  Definition env : Type := t (fgtyp * fcomponent).
-
-  (* The default type of a variable not in the typing environment *)
-  Parameter deftyp : fgtyp * fcomponent.
-
-  (* Find the type of a variable in a typing environment.
-     If a variable is not in the typing environment, return the default type. *)
-  Parameter vtyp : SE.t -> env -> (fgtyp * fcomponent).
-
-  (* Return the size of a variable in a typing environment.
-     If a variable is not in the typing environment, return the size of the
-     default type. *)
-  (* Parameter vsize : SE.t -> env -> nat. *)
-
-  Axiom find_some_vtyp :
-    forall {x : SE.t} {ty : fgtyp * fcomponent} {e : env}, find x e = Some ty -> vtyp x e = ty.
-  Axiom find_none_vtyp :
-    forall {x : SE.t} {e : env}, find x e = None -> vtyp x e = deftyp.
-  Axiom vtyp_find :
-    forall {x : SE.t} {ty : fgtyp * fcomponent} {e : env},
-      (vtyp x e == ty) = (find x e == Some ty) || ((find x e == None) && (ty == deftyp)).
-  Axiom vtyp_add_eq :
-    forall {x y : SE.t} {ty : fgtyp * fcomponent} {e : env}, x == y -> vtyp x (add y ty e) = ty.
-  Axiom vtyp_add_neq :
-    forall {x y : SE.t} {ty : fgtyp * fcomponent} {e : env},
-      x != y -> vtyp x (add y ty e) = vtyp x e.
-  (* Axiom vsize_add_eq : *)
-  (*   forall {x y : SE.t} {ty : fgtyp} {e : env}, *)
-  (*     x == y -> vsize x (add y ty e) = sizeof_fgtyp ty. *)
-  (* Axiom vsize_add_neq : *)
-  (*   forall {x y : SE.t} {ty : fgtyp} {e : env}, *)
-  (*     x != y -> vsize x (add y ty e) = vsize x e. *)
-  Axiom not_mem_vtyp :
-    forall {v : SE.t} {e : env}, ~~ mem v e -> vtyp v e = deftyp.
-  (* Axiom vtyp_vsize : *)
-  (*   forall {x : SE.t} {e : env} {ty : fgtyp}, *)
-  (*     vtyp x e = ty -> vsize x e = sizeof_fgtyp ty. *)
-
-End CmpntEnv.
-
-Module MakeCmpntEnv (V : SsrOrder) (VM : SsrFMap with Module SE := V) <:
-  CmpntEnv with Module SE := V.
-
-  Include VM.
-  Module Lemmas := FMapLemmas VM.
-
-  Definition env : Type := t (fgtyp * fcomponent).
-
-  (* The default type of a variable not in the typing environment *)
-  Definition deftyp := (Fuint 0, Node).
-
-  (* Find the type of a variable in a typing environment.
-     If a variable is not in the typing environment, return the default type. *)
-  Definition vtyp (v : V.t) (e : env) : fgtyp * fcomponent :=
-    match VM.find v e with
-    | None => deftyp
-    | Some ty => ty
-    end.
-
-  (* Return the size of a variable in a typing environment.
-     If a variable is not in the typing environment, return the size of the
-     default type. *)
-  (* Definition vsize (v : V.t) (e : env) : nat := sizeof_fgtyp (vtyp v e). *)
-
-  Lemma find_some_vtyp {x ty e} : find x e = Some ty -> vtyp x e = ty.
-  Proof. move=> H. rewrite /vtyp H. reflexivity. Qed.
-
-  Lemma find_none_vtyp {x e} : find x e = None -> vtyp x e = deftyp.
-  Proof. move=> H. rewrite /vtyp H. reflexivity. Qed.
-
-  Lemma vtyp_find {x ty e} :
-    (vtyp x e == ty) = (find x e == Some ty) || ((find x e == None) && (ty == deftyp)).
-  Proof.
-    dcase (find x e); case.
-    - move=> a Hfind. rewrite (find_some_vtyp Hfind) /= orbF. case Heq: (a == ty).
-      + by rewrite (eqP Heq) eqxx.
-      + symmetry. apply/eqP => H. case: H => H. rewrite H eqxx in Heq. discriminate.
-    - move=> Hnone. rewrite (find_none_vtyp Hnone) eqxx /=. rewrite eq_sym.
-      reflexivity.
-  Qed.
-
-  Lemma vtyp_add_eq {x y ty e} : x == y -> vtyp x (add y ty e) = ty.
-  Proof. rewrite /vtyp /add => H. by rewrite (Lemmas.find_add_eq H). Qed.
-
-  Lemma vtyp_add_neq {x y ty e} : x != y -> vtyp x (add y ty e) = vtyp x e.
-  Proof.
-    move/negP=> Hxy. rewrite /vtyp /add. by rewrite (Lemmas.find_add_neq Hxy).
-  Qed.
-
-  (* Lemma vsize_add_eq {x y ty e} : x == y -> vsize x (add y ty e) = sizeof_fgtyp ty. *)
-  (* Proof. rewrite /vsize=> H. by rewrite (vtyp_add_eq H). Qed. *)
-
-  (* Lemma vsize_add_neq {x y ty e} : x != y -> vsize x (add y ty e) = vsize x e. *)
-  (* Proof. rewrite /vsize => H. by rewrite (vtyp_add_neq H). Qed. *)
-
-  Lemma not_mem_vtyp v e : ~~ mem v e -> vtyp v e = deftyp.
-  Proof. rewrite /vtyp => H. by rewrite Lemmas.not_mem_find_none. Qed.
-
-  (* Lemma vtyp_vsize x e ty : vtyp x e = ty -> vsize x e = sizeof_fgtyp ty. *)
-  (* Proof. rewrite /vsize /vtyp. move=> ->. reflexivity. Qed. *)
-
-End MakeCmpntEnv.
-
-Module CE <: CmpntEnv := MakeCmpntEnv VarOrder VM.
 
 
