src/HiFirrtl.v
@@ -9,8 +9,6 @@ Unset Strict Implicit.
 Import Prenex Implicits.
 
 
-(*Import LoFirrtl.*)
-
 Section HiFirrtl.
 
 
@@ -24,14 +22,17 @@ Section HiFirrtl.
   
   Inductive hfexpr : Type :=
   | Econst : sign -> bits -> hfexpr
-  | Eref : var -> hfexpr
   | Ecast : ucast -> hfexpr -> hfexpr
   | Eprim_unop : eunop -> hfexpr -> hfexpr
   | Eprim_binop : ebinop -> hfexpr -> hfexpr -> hfexpr
   | Emux : hfexpr -> hfexpr -> hfexpr -> hfexpr
   | Evalidif : hfexpr -> hfexpr -> hfexpr
-  | Esubfield : hfexpr -> hfexpr -> hfexpr (* HiFirrtl *)
-  | Eaccess : hfexpr -> hfexpr -> hfexpr (* HiFirrtl *)
+  | Eref : href -> hfexpr
+  with href : Type :=
+  | Eid : var -> href
+  | Esubfield : href -> var -> href (* HiFirrtl *)
+  | Esubindex : href -> nat -> href (* HiFirrtl *)
+  | Esubaccess : href -> hfexpr -> href (* HiFirrtl *)
   .
 
   (****** Statements ******)
@@ -39,7 +40,7 @@ Section HiFirrtl.
   Record hfmem : Type :=
     mk_fmem
       {
-        mid : var;
+        (* mid : var; *)
         data_type : ftype;
         depth : nat;
         reader : seq var;
@@ -56,7 +57,7 @@ Section HiFirrtl.
   Record hfreg : Type :=
     mk_freg
       {
-        rid : var;
+        (* rid : var; *)
         type : ftype;
         clock : hfexpr;
         reset : rst
@@ -65,13 +66,13 @@ Section HiFirrtl.
   Inductive hfstmt : Type :=
   | Sskip
   | Swire : var -> ftype -> hfstmt
-  | Sreg : hfreg -> hfstmt
-  | Smem : hfmem -> hfstmt
+  | Sreg : var -> hfreg -> hfstmt
+  | Smem : var -> hfmem -> hfstmt
   | Sinst : var -> var -> hfstmt
   | Snode : var -> hfexpr -> hfstmt
-  | Sfcnct : hfexpr -> hfexpr -> hfstmt
-  | Spcnct : hfexpr -> hfexpr -> hfstmt
-  | Sinvalid : var -> hfstmt
+  | Sfcnct : href -> hfexpr -> hfstmt
+  | Spcnct : href -> hfexpr -> hfstmt
+  | Sinvalid : href -> hfstmt
   (* | Sattach : seq var -> fstmt *)
   | Swhen : hfexpr -> seq hfstmt -> seq hfstmt -> hfstmt
   | Sstop : hfexpr -> hfexpr -> nat -> hfstmt
@@ -96,7 +97,105 @@ Section HiFirrtl.
 
 End HiFirrtl.
 
-(* rhs *)
+
+(* A mapping from a variable to its component type *)
+
+Section Component_types.
+
+  Variable var : eqType.
+  
+  Inductive cmpnt_init_typs : Type :=
+  | Aggr_typ : ftype -> cmpnt_init_typs
+  | Reg_typ : hfreg var -> cmpnt_init_typs
+  | Mem_typ : hfmem var -> cmpnt_init_typs.
+
+End Component_types.
+
+Module Type CmpntEnv (V : SsrOrder) <: SsrFMap.
+  Include SsrFMap.
+
+  Local Notation var := V.t.
+  Local Notation cmpnttyp := (cmpnt_init_typs V.T).
+  Definition env : Type := t (cmpnttyp * fcomponent).
+
+  (* The default type of a variable not in the typing environment *)
+  Parameter deftyp : cmpnttyp * fcomponent.
+  (* Find the type of a variable in a typing environment.
+     If a variable is not in the typing environment, return the default type. *)
+  Parameter vtyp : SE.t -> env -> (cmpnttyp * fcomponent).
+  (* Return the size of a variable in a typing environment.
+     If a variable is not in the typing environment, return the size of the
+     default type. *)
+  (* Parameter vsize : SE.t -> env -> nat. *)
+  Axiom find_some_vtyp :
+    forall {x : SE.t} {ty :cmpnttyp * fcomponent} {e : env}, find x e = Some ty -> vtyp x e = ty.
+  Axiom find_none_vtyp :
+    forall {x : SE.t} {e : env}, find x e = None -> vtyp x e = deftyp.
+  (* Axiom vtyp_find : *)
+  (*   forall {x : SE.t} {ty : cmpnt_init_typs V.T * fcomponent} {e : env}, *)
+  (*     (vtyp x e == ty) = (find x e == Some ty) || ((find x e == None) && (ty == deftyp)). *)
+  Axiom vtyp_add_eq :
+    forall {x y : SE.t} {ty : cmpnt_init_typs V.T * fcomponent} {e : env}, x == y -> vtyp x (add y ty e) = ty.
+  Axiom vtyp_add_neq :
+    forall {x y : SE.t} {ty : cmpnt_init_typs V.T * fcomponent} {e : env},
+      x != y -> vtyp x (add y ty e) = vtyp x e.
+  (* Axiom vsize_add_eq : *)
+  (*   forall {x y : SE.t} {ty : fgtyp} {e : env}, *)
+  (*     x == y -> vsize x (add y ty e) = sizeof_fgtyp ty. *)
+  (* Axiom vsize_add_neq : *)
+  (*   forall {x y : SE.t} {ty : fgtyp} {e : env}, *)
+  (*     x != y -> vsize x (add y ty e) = vsize x e. *)
+  Axiom not_mem_vtyp :
+    forall {v : SE.t} {e : env}, ~~ mem v e -> vtyp v e = deftyp.
+  (* Axiom vtyp_vsize : *)
+  (*   forall {x : SE.t} {e : env} {ty : fgtyp}, *)
+  (*     vtyp x e = ty -> vsize x e = sizeof_fgtyp ty. *)
+
+End CmpntEnv.
+
+Module MakeCmpntEnv (V : SsrOrder) (VM : SsrFMap with Module SE := V) <:
+  CmpntEnv V with Module SE := V.
+  Include VM.
+  Module Lemmas := FMapLemmas VM.
+  Local Notation cmpnttyp := (cmpnt_init_typs V.T).
+  (* Definition aggr_typ ty := @Aggr_typ V.T ty. *)
+  (* Definition reg_typ ty := @Reg_typ V.T ty. *)
+  (* Definition mem_typ ty := @Mem_typ V.T ty. *)
+  Definition env : Type := t (cmpnttyp * fcomponent).
+
+  (* The default type of a variable not in the typing environment *)
+  Definition deftyp := (Aggr_typ V.T (Gtyp (Fuint 0)), Node).
+
+  (* Find the type of a variable in a typing environment.
+     If a variable is not in the typing environment, return the default type. *)
+  Definition vtyp (v : V.t) (e : env) : cmpnttyp * fcomponent :=
+    match VM.find v e with
+    | None => deftyp
+    | Some ty => ty
+    end.
+
+  Lemma find_some_vtyp {x ty e} : find x e = Some ty -> vtyp x e = ty.
+  Proof. move=> H. rewrite /vtyp H. reflexivity. Qed.
+
+  Lemma find_none_vtyp {x e} : find x e = None -> vtyp x e = deftyp.
+  Proof. move=> H. rewrite /vtyp H. reflexivity. Qed.
+
+  Lemma vtyp_add_eq {x y ty e} : x == y -> vtyp x (add y ty e) = ty.
+  Proof. rewrite /vtyp /add => H. by rewrite (Lemmas.find_add_eq H). Qed.
+
+  Lemma vtyp_add_neq {x y ty e} : x != y -> vtyp x (add y ty e) = vtyp x e.
+  Proof.
+    move/negP=> Hxy. rewrite /vtyp /add. by rewrite (Lemmas.find_add_neq Hxy).
+  Qed.
+
+  Lemma not_mem_vtyp v e : ~~ mem v e -> vtyp v e = deftyp.
+  Proof. rewrite /vtyp => H. by rewrite Lemmas.not_mem_find_none. Qed.
+
+End MakeCmpntEnv.
+
+Module CE (*<: CmpntEnv VarOrder *) := MakeCmpntEnv VarOrder VM.
+
+(* rhs expressions *)
 Section Rhs_expr.
   Variable tmp : eqType.
   Inductive rhs_expr : Type :=
@@ -115,7 +214,7 @@ Section Rhs_expr.
   
 End Rhs_expr.
 
-Module Type StructStore (V : SsrOrder) (CE : CmpntEnv with Module SE := V).
+Module Type StructStore (V : SsrOrder) (CE : CmpntEnv V with Module SE := V).
   Module Lemmas := FMapLemmas CE.
 
   Local Notation var := V.t.
@@ -178,7 +277,7 @@ Module StructType (V:SsrOrder)<: HasDefaultTyp.
   Definition default : t := R_default V.T.
 End StructType.
 
-Module MakeStructStore (V : SsrOrder) (CE : CmpntEnv with Module SE := V) <:
+Module MakeStructStore (V : SsrOrder) (CE : CmpntEnv V with Module SE := V) <:
   StructStore V CE.
   Module StructTypeV := StructType V.
   Include MakeTStoreMap V StructTypeV. 
@@ -192,7 +291,7 @@ Module MakeHiFirrtl
        (V : SsrOrder)
        (VS : SsrFSet with Module SE := V)
        (VM : SsrFMap with Module SE := V)
-       (CE : CmpntEnv with Module SE := V)
+       (CE : CmpntEnv V with Module SE := V)
        (SV : StructStore V CE).
   (* Local Open Scope hifirrtl. *)
   
@@ -200,35 +299,37 @@ Module MakeHiFirrtl
   Module VSLemmas := SsrFSetLemmas VS.
 
   Local Notation var := V.t.
-  
+
   Local Notation cstate := SV.t.
+  Local Notation cenv := @CE.env.
 
-
-  (* Definition fexpr := fexpr V.T. *)
-  (* Definition lofexpr e := @Lfexpr V.T e. *)
   Definition econst s c := @Econst V.T s c.
-  Definition eref v := @Eref V.T v.
   Definition ecast u e := @Ecast V.T u e.
   Definition eprim_unop u e := @Eprim_unop V.T u e.
   Definition eprim_binop b e1 e2 := @Eprim_binop V.T b e1 e2.
   Definition emux c e1 e2 := @Emux V.T c e1 e2.
   Definition evalidif c e := @Evalidif V.T c e.
   Definition hfexpr := hfexpr V.T.
-  Definition esubfield e1 e2 := @Esubfield V.T e1 e2.
-  Definition eaccess e1 e2 := @Eaccess V.T e1 e2.
+  Definition eref r := @Eref V.T r.
+  Definition eid v := @Eid V.T v.
+  Definition esubfield r v := @Esubfield V.T r v.
+  Definition esubindex r n := @Esubindex V.T r n.
+  Definition esubaccess r e := @Esubaccess V.T r e.
+  Definition href := href V.T.
 
   Definition hfstmt := hfstmt V.T.
   Definition sskip := @Sskip V.T.
   Definition swire v t := @Swire V.T v t.
-  Definition sreg r := @Sreg V.T r.
-  Definition smem m := @Smem V.T m.
+  Definition sreg v r := @Sreg V.T v r.
+  Definition smem v m := @Smem V.T v m.
   Definition snode v e := @Snode V.T v e.
   Definition sfcnct v1 v2 := @Sfcnct V.T v1 v2.
   Definition spcnct v1 v2 := @Spcnct V.T v1 v2.
   Definition sinvalid v1 := @Sinvalid V.T v1.
   Definition swhen c s1 s2 := @Swhen V.T c s1 s2.
   Definition sstop e1 e2 n := @Sstop V.T e1 e2 n.
-
+  Definition sinst v1 v2 := @Sinst V.T v1 v2.
+  
   Definition hfreg := @hfreg V.T.
   Definition mk_hfreg := @mk_freg V.T.
   Definition nrst := @NRst V.T.
@@ -278,128 +379,36 @@ Module MakeHiFirrtl
     end.
 
   (* rhs expr has right orient *)
-  Fixpoint valid_rhs_fexpr (e : hfexpr) (ce : CE.env) :=
+  Fixpoint valid_rhs_fexpr (e : hfexpr) (ce : cenv) :=
     match e with
     | Econst _ _ => true
-    | Eref v => let (_,c) := CE.vtyp v ce in valid_rhs_orient (orient_of_comp c)
+    | Eref r => valid_rhs_ref r ce
     | Ecast _ _ => true
     | Eprim_binop _ _ _ => true
     | Eprim_unop _ _ => true
     | Emux _ e1 e2 => valid_rhs_fexpr e1 ce && (valid_rhs_fexpr e2 ce)
     | Evalidif _ e => valid_rhs_fexpr e ce
-    | Esubfield e _ => valid_rhs_fexpr e ce
-    | Eaccess _ _ => true                                       
-    end.
+    end
+  with valid_rhs_ref (e : href) (ce : cenv) :=
+         match e with
+         | Eid r => let (_,c) := CE.vtyp r ce in valid_rhs_orient (orient_of_comp c)
+         | Esubfield r _ => valid_rhs_ref r ce
+         | Esubindex r _ => valid_rhs_ref r ce
+         | Esubaccess r _ => valid_rhs_ref r ce
+         end.
 
-  Definition valid_rhs (re : rhs_expr) (ce : CE.env) : bool :=
+  Definition valid_rhs (re : rhs_expr) (ce : cenv) : bool :=
     match re with
     | R_default => true
     | R_ftype t => is_passive t
     | R_fexpr e => valid_rhs_fexpr e ce
     | R_fstmt s => match s with
-                   | Sreg _ | Smem _ => true
+                   | Sreg _ _ | Smem _ _ => true
                    | _ => false
                    end
     end.
   
   (****** Semantics ******)
-
-  (** TBD. Flatten. upd ce and cs by flattened atoms in ports *)
-
-
-  Fixpoint type_of_hfexpr (e : hfexpr) (ce : CE.env) : fgtyp :=
-    match e with
-    | Econst Signed bs => Fsint (size bs)
-    | Econst Unsigned bs => Fuint (size bs)
-    | Eref v => fst (CE.vtyp v ce)
-    | Ecast AsUInt e1 => Fuint (sizeof_fgtyp (type_of_hfexpr e1 ce))
-    | Ecast AsSInt e1 => Fsint (sizeof_fgtyp (type_of_hfexpr e1 ce))
-    | Ecast AsClock e1 => Fclock
-    | Eprim_unop (Upad n) e1 => let t := type_of_hfexpr e1 ce in
-                                match t with
-                                | Fsint w => Fsint (maxn w n)
-                                | Fuint w => Fuint (maxn w n)
-                                | Fclock => Fuint 0
-                                end
-    | Eprim_unop (Ushl n) e1 => let t := type_of_hfexpr e1 ce in
-                                match t with
-                                | Fsint w => Fsint (w + n)
-                                | Fuint w => Fuint (w + n)
-                                | Fclock => Fuint 0
-                                end
-    | Eprim_unop (Ushr n) e1 => let t := type_of_hfexpr e1 ce in
-                                match t with
-                                | Fsint w => Fsint (maxn (w - n) 1)
-                                | Fuint w => Fuint (maxn (w - n) 1)
-                                | Fclock => Fuint 0
-                                end
-    | Eprim_unop Ucvt e1 => let t := type_of_hfexpr e1 ce in
-                                match t with
-                                | Fsint w => Fsint w
-                                | Fuint w => Fsint (w + 1) 
-                                | Fclock => Fuint 0
-                                end
-    | Eprim_unop Uneg e1 => Fsint (sizeof_fgtyp (type_of_hfexpr e1 ce))
-    | Eprim_unop Unot e1 => Fuint (sizeof_fgtyp (type_of_hfexpr e1 ce))
-    | Eprim_unop (Uextr n1 n2) e1 => Fuint (n1 - n2 + 1)
-    | Eprim_unop (Uhead n) e1 => Fuint n
-    | Eprim_unop (Utail n) e1 => Fuint (sizeof_fgtyp (type_of_hfexpr e1 ce) - n)
-    | Eprim_unop _ e1 => Fuint 1
-    | Eprim_binop (Bcomp _) e1 e2 => Fuint 1
-    | Eprim_binop Badd e1 e2
-    | Eprim_binop Bsub e1 e2 => let t1 := type_of_hfexpr e1 ce in
-                                let t2 := type_of_hfexpr e2 ce in
-                                match t1, t2 with
-                                | Fuint w1 , Fuint w2 => Fuint (maxn w1 w2 + 1)
-                                | Fsint w1 , Fsint w2 => Fsint (maxn w1 w2 + 1)
-                                | _, _ => Fuint 0
-                                end
-    | Eprim_binop Bmul e1 e2 => let t1 := type_of_hfexpr e1 ce in
-                                let t2 := type_of_hfexpr e2 ce in
-                                match t1, t2 with
-                                | Fuint w1 , Fuint w2 => Fuint (w1 + w2)
-                                | Fsint w1 , Fsint w2 => Fsint (w1 + w2)
-                                | _, _ => Fuint 0
-                                end
-    | Eprim_binop Bdiv e1 e2
-    | Eprim_binop Bsdiv e1 e2 => let t1 := type_of_hfexpr e1 ce in
-                                 let t2 := type_of_hfexpr e2 ce in
-                                 match t1, t2 with
-                                 | Fuint w1 , Fuint w2 => Fuint w1
-                                 | Fsint w1 , Fsint w2 => Fsint (w1 + 1)
-                                 | _, _ => Fuint 0
-                                 end
-    | Eprim_binop Brem e1 e2
-    | Eprim_binop Bsrem e1 e2 => let t1 := type_of_hfexpr e1 ce in
-                                 let t2 := type_of_hfexpr e2 ce in
-                                 match t1, t2 with
-                                 | Fuint w1 , Fuint w2 => Fuint (minn w1 w2)
-                                 | Fsint w1 , Fsint w2 => Fsint (minn w1 w2)
-                                 | _, _ => Fuint 0
-                                 end
-    | Eprim_binop Bdshl e1 e2 => let t1 := type_of_hfexpr e1 ce in
-                                 let t2 := type_of_hfexpr e2 ce in
-                                 match t1, t2 with
-                                 | Fuint w1 , Fuint w2 => Fuint (w1 + 2 ^ w2 - 1)
-                                 | Fsint w1 , Fuint w2 => Fsint (w1 + 2 ^ w2 - 1)
-                                 | _, _ => Fuint 0
-                                 end
-    | Eprim_binop Bdshr e1 e2 => let t1 := type_of_hfexpr e1 ce in
-                                 let t2 := type_of_hfexpr e2 ce in
-                                 match t1, t2 with
-                                 | Fuint w1 , Fuint w2 => Fuint w1
-                                 | Fsint w1 , Fuint w2 => Fsint w1
-                                 | _, _ => Fuint 0
-                                 end
-    | Eprim_binop _ e1 e2 => let t1 := type_of_hfexpr e1 ce in
-                             let t2 := type_of_hfexpr e2 ce in
-                             Fuint (maxn (sizeof_fgtyp t1) (sizeof_fgtyp t2))
-    | Emux c e1 e2 => let t1 := type_of_hfexpr e1 ce in
-                      let t2 := type_of_hfexpr e2 ce in
-                      Fuint (maxn (sizeof_fgtyp t1) (sizeof_fgtyp t2))
-    | Evalidif c e1 => type_of_hfexpr e1 ce
-    | Esubfield _ _ | Eaccess _ _ => Fuint 0
-    end.
 
   (* ground type equivalence *)
   Definition fgtyp_equiv t1 t2 :=
@@ -410,223 +419,579 @@ Module MakeHiFirrtl
     | _, _ => false
     end.
 
-  Definition change_width t s:=
-    match t with
-    | Fuint _ => Fuint s
-    | Fsint _ => Fsint s
-    | Clock => Clock
+  Fixpoint ftype_equiv t1 t2 :=
+    match t1, t2 with
+    | Gtyp gt1, Gtyp gt2 => fgtyp_equiv gt1 gt2
+    | Atyp t1 n1, Atyp t2 n2 => (n1 == n2) && ftype_equiv t1 t2
+    | Btyp bt1, Btyp bt2 => fbtyp_equiv bt1 bt2
+    | _, _ => false
+    end
+  with fbtyp_equiv bt1 bt2 :=
+         match bt1, bt2 with
+         | Fnil, Fnil => true
+         | Fflips v1 Flipped t1 fs1, Fflips v2 Flipped t2 fs2 =>
+           (v1 == v2) && ftype_equiv t1 t2 && fbtyp_equiv fs1 fs2
+         | Fflips v1 Nflip t1 fs1, Fflips v2 Nflip t2 fs2 =>
+           (v1 == v2) && ftype_equiv t1 t2 && fbtyp_equiv fs1 fs2
+         | _, _ => false
+         end.
+  
+
+  (** Pass Resolvekinds *)
+  (** Pass InferType *)
+
+  Definition aggr_typ t := @Aggr_typ V.T t.
+  Definition reg_typ t := @Reg_typ V.T t.
+  Definition mem_typ t := @Mem_typ V.T t.
+
+  
+  (* Resolve compnent kind and init type from statement *)
+  Inductive resolveKinds_stmt : hfstmt -> cenv -> cenv -> Prop :=
+  | Resolve_wire v t (ce : cenv) (ce' : cenv) :
+      CELemmas.P.Add v (aggr_typ t, Wire) ce ce' ->
+      resolveKinds_stmt (swire v t) ce ce'
+  | Resolve_reg v r ce ce' :
+      CELemmas.P.Add v (reg_typ r, Register) ce ce' ->
+      resolveKinds_stmt (sreg v r) ce ce'
+  | Resolve_inst v1 v2 ce ce' :
+       CELemmas.P.Add v1 (fst (CE.vtyp v2 ce), Instanceof) ce ce' ->
+       resolveKinds_stmt (sinst v1 v2) ce ce'
+  | Resolve_node v e ce ce' :
+      CELemmas.P.Add v CE.deftyp ce ce' ->
+      resolveKinds_stmt (snode v e) ce ce'
+  | Resolve_mem v m ce ce' :
+      CELemmas.P.Add v (mem_typ m, Memory) ce ce' ->
+      resolveKinds_stmt (smem v m) ce ce'
+  .
+
+  Inductive resolveKinds_port : hfport -> CE.env -> CE.env -> Prop :=
+  | Resolve_input v t ce ce' :
+      CELemmas.P.Add v (aggr_typ t, In_port) ce ce' ->
+      resolveKinds_port (hinport v t) ce ce'
+  | Resolve_output v t ce ce' :
+      CELemmas.P.Add v (aggr_typ t, Out_port) ce ce' ->
+      resolveKinds_port (houtport v t) ce ce'
+  .
+
+  (** decide the type and width of hifirrtl expressions *)
+
+  Parameter v2var : V.t -> Var.var.
+
+  Definition def_ftype := Gtyp (Fuint 0).
+  
+  Fixpoint mux_types t1 t2 : ftype :=
+      match t1, t2 with
+      | Gtyp (Fuint w1), Gtyp (Fuint w2) => (Gtyp (Fuint (maxn w1 w2)))
+      | Gtyp (Fsint w1), Gtyp (Fsint w2) => (Gtyp (Fsint (maxn w1 w2)))
+      | Gtyp Fclock, Gtyp Fclock => (Gtyp Fclock)
+      | Atyp t1 n1, Atyp t2 n2 => if n1 == n2 then (Atyp (mux_types t1 t2) n1)
+                                  else def_ftype
+      | Btyp bs1, Btyp bs2 => Btyp (mux_btyps bs1 bs2)
+      | _, _ => def_ftype
+      end
+  with mux_btyps bs1 bs2 : ffield :=
+         match bs1, bs2 with
+         | Fnil, Fnil => (Fnil)
+         | Fflips v1 Flipped t1 fs1, Fflips v2 Flipped t2 fs2 =>
+           if v1 == v2 then
+             (Fflips v1 Flipped (mux_types t1 t2) (mux_btyps fs1 fs2))
+           else Fnil
+         | Fflips v1 Nflip t1 fs1, Fflips v2 Nflip t2 fs2 =>
+           if v1 == v2 then
+             (Fflips v1 Flipped (mux_types t1 t2) (mux_btyps fs1 fs2))
+           else Fnil
+         | _, _ => Fnil
     end.
 
+  Definition type_of_cmpnttyp ct :=
+    match ct with
+    | Aggr_typ t => t
+    | Reg_typ r => @type V.T r
+    | Mem_typ m => @data_type V.T m
+    end.
+  
+  Fixpoint type_of_hfexpr (e : hfexpr) (ce : cenv) : ftype :=
+    match e with
+    | Econst Signed bs => Gtyp (Fsint (size bs))
+    | Econst Unsigned bs => Gtyp (Fuint (size bs))
+    | Eref r => type_of_ref r ce
+    | Ecast AsUInt e1 => let t := type_of_hfexpr e1 ce in
+                         match t with
+                         | Gtyp (Fsint w) | Gtyp (Fuint w) => Gtyp (Fuint w)
+                         | Gtyp Fclock => Gtyp (Fuint 1)
+                         | _ => def_ftype
+                         end
+    | Ecast AsSInt e1 => let t := type_of_hfexpr e1 ce in
+                         match t with
+                         | Gtyp (Fsint w) | Gtyp (Fuint w) => Gtyp (Fsint w)
+                         | Gtyp Fclock => Gtyp (Fsint 1)
+                         | _ => def_ftype
+                         end
+    | Ecast AsClock e1 => let t := type_of_hfexpr e1 ce in
+                          match t with
+                          | Gtyp _ =>  Gtyp Fclock
+                          | _ => def_ftype
+                          end
+    | Eprim_unop (Upad n) e1 => let t := type_of_hfexpr e1 ce in
+                                match t with
+                                | Gtyp (Fsint w) => Gtyp (Fsint (maxn w n))
+                                | Gtyp (Fuint w) => Gtyp (Fuint (maxn w n))
+                                | _ => def_ftype
+                                end
+    | Eprim_unop (Ushl n) e1 => let t := type_of_hfexpr e1 ce in
+                                match t with
+                                | Gtyp (Fsint w) => Gtyp (Fsint (w + n))
+                                | Gtyp (Fuint w) => Gtyp (Fuint (w + n))
+                                | _ => def_ftype
+                                end
+    | Eprim_unop (Ushr n) e1 => let t := type_of_hfexpr e1 ce in
+                                match t with
+                                | Gtyp (Fsint w) => Gtyp (Fsint (maxn (w - n) 1))
+                                | Gtyp (Fuint w) => Gtyp (Fuint (maxn (w - n) 1))
+                                | _ => def_ftype
+                                end
+    | Eprim_unop Ucvt e1 => let t := type_of_hfexpr e1 ce in
+                                match t with
+                                | Gtyp (Fsint w) => Gtyp (Fsint w)
+                                | Gtyp (Fuint w) => Gtyp (Fsint (w + 1))
+                                | _ => def_ftype
+                                end
+    | Eprim_unop Uneg e1 => let t := type_of_hfexpr e1 ce in
+                                match t with
+                                | Gtyp (Fsint w) | Gtyp (Fuint w) => Gtyp (Fsint w)
+                                | _ => def_ftype
+                                end
+    | Eprim_unop Unot e1 => let t := type_of_hfexpr e1 ce in
+                                match t with
+                                | Gtyp (Fsint w) | Gtyp (Fuint w) => Gtyp (Fuint w)
+                                | _ => def_ftype
+                                end
+    | Eprim_unop (Uextr n1 n2) e1 => let t := type_of_hfexpr e1 ce in
+                                     match t with
+                                     | Gtyp (Fsint _) | Gtyp (Fuint _) => Gtyp (Fuint (n1 - n2 + 1))
+                                     | _ => def_ftype
+                                     end
+    | Eprim_unop (Uhead n) e1 => let t := type_of_hfexpr e1 ce in
+                                 match t with
+                                 | Gtyp (Fsint _) | Gtyp (Fuint _) => Gtyp (Fuint n)
+                                 | _ => def_ftype
+                                 end
+    | Eprim_unop (Utail n) e1 => let t := type_of_hfexpr e1 ce in
+                                 match t with
+                                 | Gtyp (Fsint w) | Gtyp (Fuint w) => Gtyp (Fuint (w - n))
+                                 | _ => def_ftype
+                                 end
+    | Eprim_unop _ e1 => let t := type_of_hfexpr e1 ce in
+                         match t with
+                         | Gtyp (Fsint _) | Gtyp (Fuint _) => Gtyp (Fuint 1)
+                         | _ => def_ftype
+                         end
+    | Eprim_binop (Bcomp _) e1 e2 => let t1 := type_of_hfexpr e1 ce in
+                                     let t2 := type_of_hfexpr e2 ce in
+                                     match t1, t2 with
+                                     | Gtyp (Fsint _), Gtyp (Fsint _)
+                                     | Gtyp (Fuint _), Gtyp (Fuint _) => Gtyp (Fuint 1)
+                                     | _, _ => def_ftype
+                                     end
+    | Eprim_binop Badd e1 e2
+    | Eprim_binop Bsub e1 e2 => let t1 := type_of_hfexpr e1 ce in
+                                let t2 := type_of_hfexpr e2 ce in
+                                match t1, t2 with
+                                | Gtyp (Fuint w1) , Gtyp (Fuint w2) => Gtyp (Fuint (maxn w1 w2 + 1))
+                                | Gtyp (Fsint w1) , Gtyp (Fsint w2) => Gtyp (Fsint (maxn w1 w2 + 1))
+                                | _, _ => def_ftype
+                                end
+    | Eprim_binop Bmul e1 e2 => let t1 := type_of_hfexpr e1 ce in
+                                let t2 := type_of_hfexpr e2 ce in
+                                match t1, t2 with
+                                | Gtyp (Fuint w1) , Gtyp (Fuint w2) => Gtyp (Fuint (w1 + w2))
+                                | Gtyp (Fsint w1) , Gtyp (Fsint w2) => Gtyp (Fsint (w1 + w2))
+                                | _, _ => def_ftype
+                                end
+    | Eprim_binop Bdiv e1 e2
+    | Eprim_binop Bsdiv e1 e2 => let t1 := type_of_hfexpr e1 ce in
+                                 let t2 := type_of_hfexpr e2 ce in
+                                 match t1, t2 with
+                                 | Gtyp (Fuint w1), Gtyp (Fuint w2) => Gtyp (Fuint w1)
+                                 | Gtyp (Fsint w1), Gtyp (Fsint w2) => Gtyp (Fsint (w1 + 1))
+                                 | _, _ => def_ftype
+                                 end
+    | Eprim_binop Brem e1 e2
+    | Eprim_binop Bsrem e1 e2 => let t1 := type_of_hfexpr e1 ce in
+                                 let t2 := type_of_hfexpr e2 ce in
+                                 match t1, t2 with
+                                 | Gtyp (Fuint w1), Gtyp (Fuint w2) => Gtyp (Fuint (minn w1 w2))
+                                 | Gtyp (Fsint w1), Gtyp (Fsint w2) => Gtyp (Fsint (minn w1 w2))
+                                 | _, _ => def_ftype
+                                 end
+    | Eprim_binop Bdshl e1 e2 => let t1 := type_of_hfexpr e1 ce in
+                                 let t2 := type_of_hfexpr e2 ce in
+                                 match t1, t2 with
+                                 | Gtyp (Fuint w1), Gtyp (Fuint w2) => Gtyp (Fuint (w1 + 2 ^ w2 - 1))
+                                 | Gtyp (Fsint w1), Gtyp (Fuint w2) => Gtyp (Fsint (w1 + 2 ^ w2 - 1))
+                                 | _, _ => def_ftype
+                                 end
+    | Eprim_binop Bdshr e1 e2 => let t1 := type_of_hfexpr e1 ce in
+                                 let t2 := type_of_hfexpr e2 ce in
+                                 match t1, t2 with
+                                 | Gtyp (Fuint w1), Gtyp (Fuint w2) => Gtyp (Fuint w1)
+                                 | Gtyp (Fsint w1), Gtyp (Fuint w2) => Gtyp (Fsint w1)
+                                 | _, _ => def_ftype
+                                 end
+    | Eprim_binop Bcat e1 e2 => let t1 := type_of_hfexpr e1 ce in
+                                let t2 := type_of_hfexpr e2 ce in
+                                match t1, t2 with
+                                | Gtyp (Fuint w1), Gtyp (Fuint w2) => Gtyp (Fuint (w1 + w2))
+                                | Gtyp (Fsint w1), Gtyp (Fuint w2) => Gtyp (Fuint (w1 + w2))
+                                | _, _ => def_ftype
+                                end
+    | Eprim_binop Band e1 e2
+    | Eprim_binop Bor e1 e2
+    | Eprim_binop Bxor e1 e2 => let t1 := type_of_hfexpr e1 ce in 
+                                let t2 := type_of_hfexpr e2 ce in
+                                match t1, t2 with
+                                | Gtyp (Fuint w1), Gtyp (Fuint w2) => Gtyp (Fuint (maxn w1 w2))
+                                | Gtyp (Fsint w1), Gtyp (Fuint w2) => Gtyp (Fuint (maxn w1 w2))
+                                | _, _ => def_ftype
+                                end
+    | Emux c e1 e2 => let t1 := type_of_hfexpr e1 ce in
+                      let t2 := type_of_hfexpr e2 ce in
+                      mux_types t1 t2 
+    | Evalidif c e1 => type_of_hfexpr e1 ce
+    end
+  with type_of_ref r ce : ftype :=
+         match r with
+         | Eid v => type_of_cmpnttyp (fst (CE.vtyp v ce))
+         | Esubfield r v => let t := type_of_ref r ce in
+                            match t with
+                            | Btyp fs => let fix aux fx := (
+                                               match fx with
+                                               | Fflips v' f t fxs => 
+                                                 if (v2var v == v') then t
+                                                 else aux fxs
+                                               | Fnil => def_ftype
+                                               end )
+                                         in aux fs
+                            | _ => def_ftype
+                            end
+         | Esubindex r n => let t := type_of_ref r ce in
+                            match t with
+                            | Atyp ty n => ty
+                            | _ => def_ftype
+                            end
+         | Esubaccess r e => let t := type_of_ref r ce in
+                            match t with
+                            | Atyp ty n => ty
+                            | _ => def_ftype
+                            end
+         end.
+
+  Definition upd_regtyp t r :=
+    mk_hfreg t (clock r) (reset r).
+  
+  Definition upd_memtyp t m :=
+    mk_hfmem t (depth m) (reader m) (writer m) (read_latency m) (write_latency m) (read_write m).
+
+  Definition is_bundle t :=
+    match t with Btyp _ => true | _ => false end.
+  
+  Definition is_vector t :=
+    match t with Atyp _ _ => true | _ => false end.
+
+  Fixpoint max_width t1 t2 :=
+    match t1, t2 with
+    | Gtyp (Fsint w1), Gtyp (Fsint w2) => Gtyp (Fsint (maxn w1 w2))
+    | Gtyp (Fuint w1), Gtyp (Fuint w2) => Gtyp (Fuint (maxn w1 w2))
+    | Atyp tn1 n1, Atyp tn2 n2 => if n2 <= n1 then Atyp (max_width tn1 tn2) n1
+                                  else t1
+    | Btyp bt1, Btyp bt2 => Btyp (max_width_f bt1 bt2)
+    | _, _ => t1
+    end
+  with max_width_f bt1 bt2 :=
+         match bt1, bt2 with
+         | Fnil, Fnil => Fnil
+         | Fflips v1 ft1 t1 fs1, Fflips v2 ft2 t2 fs2 =>
+           Fflips v1 ft1 (max_width t1 t2) (max_width_f fs1 fs2)
+         | Fnil, _ => bt1
+         | f, Fnil => f
+         end.
+
+  Fixpoint upd_name_ftype ft v t : ftype :=
+    match ft with
+    | Gtyp gt => ft
+    | Atyp tn n => Atyp (upd_name_ftype tn v t) n
+    | Btyp bt => Btyp (upd_name_ffield bt v t)
+    end
+  with upd_name_ffield bt v t : ffield :=
+         match bt with
+         | Fnil => Fnil
+         | Fflips v1 ft t1 fs => if v1 == v then Fflips v1 ft (max_width t1 t) fs
+                                 else Fflips v1 ft (upd_name_ftype t1 v t)
+                                             (upd_name_ffield fs v t)
+         end.
+  
+  Definition upd_cmpnttyp_field ft v t :=
+    match ft with
+    | Reg_typ r => Reg_typ (upd_regtyp (upd_name_ftype (type r) v t) r)
+    | Mem_typ m => Mem_typ (upd_memtyp (upd_name_ftype (data_type m) v t) m)
+    | Aggr_typ ft => @Aggr_typ V.T (upd_name_ftype ft v t)
+    end.
+  
+  (* esubfield r v , type_of_ref *)
+  Fixpoint upd_subfield_typ r v t ce :=
+    match r with
+    (* v1.v *)
+    | Eid v1 => CE.add v1 (upd_cmpnttyp_field (fst (CE.vtyp v1 ce)) v t, snd (CE.vtyp v1 ce)) ce
+    (* r1.v1.v *)
+    | Esubfield r1 v1 => upd_subfield_typ r1 v t ce
+    | _ => ce
+    end.
+  
+  (** Pass InferTypes & InferWidth *)
+  
+  Inductive inferTypeAndWidth : hfstmt -> cenv -> cenv -> Prop :=
+  (* node *)
+  | Infer_node v e ce ce' :
+      CELemmas.P.Add v (aggr_typ (type_of_hfexpr e ce), Node) ce ce' ->
+      inferTypeAndWidth (snode v e) ce ce'
+  (* full connect to reg *)
+  | Infer_connect_reg v ty e ce ce' :
+      CE.find v ce = Some (reg_typ ty, Register) ->
+      ftype_equiv (type ty) (type_of_hfexpr e ce) ->
+      CELemmas.P.Add v (reg_typ (upd_regtyp (type_of_hfexpr e ce) ty), Register) ce ce' ->
+      inferTypeAndWidth (sfcnct (eid v) e) ce ce'
+  (* full connect to mem *)
+  | Infer_connect_mem v ty e ce ce' :
+      CE.find v ce = Some (mem_typ ty, Memory) ->
+      ftype_equiv (data_type ty) (type_of_hfexpr e ce) ->
+      CELemmas.P.Add v (mem_typ (upd_memtyp (type_of_hfexpr e ce) ty), Memory) ce ce' ->
+      inferTypeAndWidth (sfcnct (eid v) e) ce ce'
+  (* full connect to ref of ports, wire and node *)
+  | Infer_connect v ty c e ce ce' :
+      CE.find v ce = Some (aggr_typ ty, c) ->
+      ftype_equiv ty (type_of_hfexpr e ce) ->
+      CELemmas.P.Add v (aggr_typ (type_of_hfexpr e ce), Wire) ce ce' ->
+      inferTypeAndWidth (sfcnct (eid v) e) ce ce'
+  (* full connect to subfield of _ *)
+  | Infer_connect_subfield r v e ce :
+      is_bundle (type_of_ref r ce) ->
+      ftype_equiv (type_of_ref (esubfield r v) ce) (type_of_hfexpr e ce) ->
+      inferTypeAndWidth (sfcnct (esubfield r v) e) ce (upd_subfield_typ r (v2var v) (type_of_hfexpr e ce) ce)
+  (* full connect to subindex of _  *)
+  | Infer_connect_subindex r n e ce ce' :                 
+      is_vector (type_of_ref r ce) ->
+      ftype_equiv (type_of_ref (esubindex r n) ce) (type_of_hfexpr e ce) ->
+      inferTypeAndWidth (sfcnct (esubindex r n) e) ce ce'
+  .
 
   (* TBD *)
   Parameter new_vecvar : var -> nat -> var.
   Parameter new_bdvar : var -> Var.var -> var.
-
   
   (** semantics of declaim  ports *)
-  Inductive eval_port : hfport -> CE.env -> cstate -> CE.env -> cstate -> Prop :=
-  (* in, ground type *)
-  | Eval_inport_gt v t ce cs ce' cs': 
-      CELemmas.P.Add v (t, In_port) ce ce' ->
-      SV.Upd v (r_ftype (Gtyp t)) cs cs' ->
-      eval_port (Finput v (Gtyp t)) ce cs ce' cs'
-  (* in, vector type *)
-  | Eval_inport_at v t n ce cs ce' cs' ce'' cs'': 
-      0 < n ->
-      eval_port (Finput (new_vecvar v n) t) ce cs ce'' cs'' ->
-      eval_port (Finput v (Atyp t n.-1)) ce' cs' ce'' cs'' ->
-      eval_port (Finput v (Atyp t n)) ce cs ce'' cs''
-  (* in, bundle type non flip *)
-  | Eval_inport_bt_nf v vt t fs n ce cs ce' cs' ce'' cs'': 
-      0 < n ->
-      eval_port (Finput (new_bdvar v vt) t) ce cs ce'' cs'' ->
-      eval_port (Finput v (Btyp fs)) ce' cs' ce'' cs'' ->
-      eval_port (Finput v (Btyp (Fflips vt Nflip t fs))) ce cs ce'' cs''
-  (* in, bundle type flip *)
-  | Eval_inport_bt_f v vt t fs n ce cs ce' cs' ce'' cs'': 
-      0 < n ->
-      eval_port (Foutput (new_bdvar v vt) t) ce cs ce'' cs'' ->
-      eval_port (Finput v (Btyp fs)) ce' cs' ce'' cs'' ->
-      eval_port (Finput v (Btyp (Fflips vt Flipped t fs))) ce cs ce'' cs''
-  (* out, ground type *)
-  | Eval_outport_gt v t ce cs ce' cs': 
-      CELemmas.P.Add v (t, In_port) ce ce' ->
-      SV.Upd v (r_ftype (Gtyp t)) cs cs' ->
-      eval_port (Foutput v (Gtyp t)) ce cs ce' cs'
-  (* out, vector type *)
-  | Eval_outport_at v t n ce cs ce' cs' ce'' cs'': 
-      0 < n ->
-      eval_port (Foutput (new_vecvar v n) t) ce cs ce'' cs'' ->
-      eval_port (Foutput v (Atyp t n.-1)) ce' cs' ce'' cs'' ->
-      eval_port (Foutput v (Atyp t n)) ce cs ce'' cs''
-  (* out, bundle type *)
-  | Eval_outport_bt_nf v vt t fs n ce cs ce' cs' ce'' cs'': 
-      0 < n ->
-      eval_port (Foutput (new_bdvar v vt) t) ce cs ce'' cs'' ->
-      eval_port (Foutput v (Btyp fs)) ce' cs' ce'' cs'' ->
-      eval_port (Foutput v (Btyp (Fflips vt Nflip t fs))) ce cs ce'' cs''
-  (* out, bundle type flip *)
-  | Eval_outport_bt_f v vt t fs n ce cs ce' cs' ce'' cs'': 
-      0 < n ->
-      eval_port (Finput (new_bdvar v vt) t) ce cs ce'' cs'' ->
-      eval_port (Foutput v (Btyp fs)) ce' cs' ce'' cs'' ->
-      eval_port (Foutput v (Btyp (Fflips vt Flipped t fs))) ce cs ce'' cs''
-  .
+  (* Inductive eval_port : hfport -> CE.env -> cstate -> CE.env -> cstate -> Prop := *)
+  (* (* in, ground type *) *)
+  (* | Eval_inport_gt v t ce cs ce' cs':  *)
+  (*     CELemmas.P.Add v (t, In_port) ce ce' -> *)
+  (*     SV.Upd v (r_ftype (Gtyp t)) cs cs' -> *)
+  (*     eval_port (Finput v (Gtyp t)) ce cs ce' cs' *)
+  (* (* in, vector type *) *)
+  (* | Eval_inport_at v t n ce cs ce' cs' ce'' cs'':  *)
+  (*     0 < n -> *)
+  (*     eval_port (Finput (new_vecvar v n) t) ce cs ce'' cs'' -> *)
+  (*     eval_port (Finput v (Atyp t n.-1)) ce' cs' ce'' cs'' -> *)
+  (*     eval_port (Finput v (Atyp t n)) ce cs ce'' cs'' *)
+  (* (* in, bundle type non flip *) *)
+  (* | Eval_inport_bt_nf v vt t fs n ce cs ce' cs' ce'' cs'':  *)
+  (*     0 < n -> *)
+  (*     eval_port (Finput (new_bdvar v vt) t) ce cs ce'' cs'' -> *)
+  (*     eval_port (Finput v (Btyp fs)) ce' cs' ce'' cs'' -> *)
+  (*     eval_port (Finput v (Btyp (Fflips vt Nflip t fs))) ce cs ce'' cs'' *)
+  (* (* in, bundle type flip *) *)
+  (* | Eval_inport_bt_f v vt t fs n ce cs ce' cs' ce'' cs'':  *)
+  (*     0 < n -> *)
+  (*     eval_port (Foutput (new_bdvar v vt) t) ce cs ce'' cs'' -> *)
+  (*     eval_port (Finput v (Btyp fs)) ce' cs' ce'' cs'' -> *)
+  (*     eval_port (Finput v (Btyp (Fflips vt Flipped t fs))) ce cs ce'' cs'' *)
+  (* (* out, ground type *) *)
+  (* | Eval_outport_gt v t ce cs ce' cs':  *)
+  (*     CELemmas.P.Add v (t, In_port) ce ce' -> *)
+  (*     SV.Upd v (r_ftype (Gtyp t)) cs cs' -> *)
+  (*     eval_port (Foutput v (Gtyp t)) ce cs ce' cs' *)
+  (* (* out, vector type *) *)
+  (* | Eval_outport_at v t n ce cs ce' cs' ce'' cs'':  *)
+  (*     0 < n -> *)
+  (*     eval_port (Foutput (new_vecvar v n) t) ce cs ce'' cs'' -> *)
+  (*     eval_port (Foutput v (Atyp t n.-1)) ce' cs' ce'' cs'' -> *)
+  (*     eval_port (Foutput v (Atyp t n)) ce cs ce'' cs'' *)
+  (* (* out, bundle type *) *)
+  (* | Eval_outport_bt_nf v vt t fs n ce cs ce' cs' ce'' cs'':  *)
+  (*     0 < n -> *)
+  (*     eval_port (Foutput (new_bdvar v vt) t) ce cs ce'' cs'' -> *)
+  (*     eval_port (Foutput v (Btyp fs)) ce' cs' ce'' cs'' -> *)
+  (*     eval_port (Foutput v (Btyp (Fflips vt Nflip t fs))) ce cs ce'' cs'' *)
+  (* (* out, bundle type flip *) *)
+  (* | Eval_outport_bt_f v vt t fs n ce cs ce' cs' ce'' cs'':  *)
+  (*     0 < n -> *)
+  (*     eval_port (Finput (new_bdvar v vt) t) ce cs ce'' cs'' -> *)
+  (*     eval_port (Foutput v (Btyp fs)) ce' cs' ce'' cs'' -> *)
+  (*     eval_port (Foutput v (Btyp (Fflips vt Flipped t fs))) ce cs ce'' cs'' *)
+  (* . *)
   
-  Inductive eval_ports : seq hfport -> CE.env -> cstate -> CE.env -> cstate -> Prop :=
-  | Eval_ports_nil ce cs : eval_ports [::] ce cs ce cs
-  | Eval_ports_cons p ps ce cs ce' cs' ce'' cs'':
-      eval_port p ce cs ce' cs' ->
-      eval_ports ps ce' cs' ce'' cs'' ->
-      eval_ports (p :: ps) ce cs ce'' cs''
-  .
+  (* Inductive eval_ports : seq hfport -> CE.env -> cstate -> CE.env -> cstate -> Prop := *)
+  (* | Eval_ports_nil ce cs : eval_ports [::] ce cs ce cs *)
+  (* | Eval_ports_cons p ps ce cs ce' cs' ce'' cs'': *)
+  (*     eval_port p ce cs ce' cs' -> *)
+  (*     eval_ports ps ce' cs' ce'' cs'' -> *)
+  (*     eval_ports (p :: ps) ce cs ce'' cs'' *)
+  (* . *)
   
-  (** semantics of single statement, update CE.env (var -> fgtyp * fcomponent) and cstate (var -> rhs_expr) *)
+  (* (** semantics of single statement, update CE.env (var -> fgtyp * fcomponent) and cstate (var -> rhs_expr) *) *)
 
   
-  Inductive eval_fstmt_single : hfstmt -> CE.env -> cstate -> CE.env -> cstate -> Prop :=
-  | Eval_sskip : forall ce cs, eval_fstmt_single sskip ce cs ce cs
-  (* declare wire with ground type *)
-  | Eval_swire_gt v t ce cs ce' cs':
-      CELemmas.P.Add v (t, Wire) ce ce' ->
-      SV.Upd v (r_ftype (Gtyp t)) cs cs' ->
-      eval_fstmt_single (swire v (Gtyp t)) ce cs ce' cs'
-  (* declare wire with vector type *)
-  | Eval_swire_agt v t n ce cs ce' cs' ce'' cs'':
-      0 < n ->
-      eval_fstmt_single (swire (new_vecvar v n) t) ce cs ce' cs' ->
-      eval_fstmt_single (swire v (Atyp t n.-1)) ce' cs' ce'' cs'' ->
-      eval_fstmt_single (swire v (Atyp t n)) ce cs ce'' cs''
-  (* TBD. declare wire with bundle type *)
-  (*| Eval_swire_bt *)
-  (* declare node with expr, valid rhs *)
-  | Eval_snode v e ce cs ce' cs':
-      valid_rhs_fexpr e ce' ->
-      CELemmas.P.Add v ((type_of_hfexpr e ce), Node) ce ce' ->
-      SV.Upd v (r_fexpr e) cs cs' ->
-      eval_fstmt_single (snode v e) ce cs ce' cs'
-  (* define full connection *)
-  (* valid flow orient, type eq between dst and src, dst width upd to max (current size, src) *)
-  | Eval_sfcnct v e ce ce' cs cs':
-      valid_lhs_orient (orient_of_comp (snd (CE.vtyp v ce))) ->
-      valid_rhs_fexpr e ce ->
-      fgtyp_equiv (fst (CE.vtyp v ce)) (type_of_hfexpr e ce) ->
-      CELemmas.P.Add v (change_width (fst (CE.vtyp v ce)) (maxn (sizeof_fgtyp (fst (CE.vtyp v ce))) (sizeof_fgtyp (type_of_hfexpr e ce))), snd (CE.vtyp v ce)) ce ce' ->
-      SV.Upd v (r_fexpr e) cs cs' ->
-      eval_fstmt_single (sfcnct (Eref v) e) ce cs ce' cs'
-  (* declare reg with ground type , reset expr type equiv with reg type*)
-  | Eval_sreg_r_gt r t c rc rs ce cs ce' cs' :
-      fgtyp_equiv (type_of_hfexpr rs ce) t ->
-      CELemmas.P.Add r (t , Register) ce ce' ->
-      SV.Upd r (r_fstmt (sreg (mk_hfreg r (Gtyp t) c (rrst rc rs)))) cs cs' ->
-      eval_fstmt_single (sreg (mk_hfreg r (Gtyp t) c (rrst rc rs))) ce cs ce' cs'
-  (* declare reg with ground type, non reset *)
-  | Eval_sreg_nr_gt r t c ce cs ce' cs' :
-      CELemmas.P.Add r (t , Register) ce ce' ->
-      SV.Upd r (r_fstmt (sreg (mk_hfreg r (Gtyp t) c nrst))) cs cs' ->
-      eval_fstmt_single (sreg (mk_hfreg r (Gtyp t) c nrst)) ce cs ce' cs'
-  (* declare reg with vector ground type *)
-  | Eval_sreg_agt r t n c rs ce cs ce' cs' ce'' cs'' :
-      0 < n ->
-      eval_fstmt_single (sreg (mk_hfreg r t c rs)) ce cs ce' cs' ->
-      eval_fstmt_single (sreg (mk_hfreg r (Atyp t n.-1) c rs)) ce' cs' ce'' cs'' ->
-      eval_fstmt_single (sreg (mk_hfreg r (Atyp t n) c rs)) ce cs ce'' cs''
-  (* declare mem with ground type *)
-  | Eval_smem_gt m t dp r w rl wl rw ce cs ce' cs' :
-      is_passive (Gtyp t) ->
-      CELemmas.P.Add m (t, Memory) ce ce' ->
-      SV.Upd m (r_fstmt (smem (mk_hfmem m (Gtyp t) dp r w rl wl rw))) cs cs' ->
-      eval_fstmt_single (smem (mk_hfmem m (Gtyp t) dp r w rl wl rw)) ce cs ce' cs'
-  (* declare mem with vector ground type *)
-  | Eval_smem_agt m t n dp r w rl wl rw ce cs ce' cs' ce'' cs'':
-      0 < n ->
-      is_passive (Atyp (Gtyp t) n) ->
-      CELemmas.P.Add m (t, Memory) ce ce' ->
-      SV.Upd (new_vecvar m n) (r_fstmt (smem (mk_hfmem m (Gtyp t) dp r w rl wl rw))) cs cs' ->
-      eval_fstmt_single (smem (mk_hfmem m (Atyp (Gtyp t) n.-1) dp r w rl wl rw)) ce' cs' ce'' cs'' ->
-      eval_fstmt_single (smem (mk_hfmem m (Atyp (Gtyp t) n) dp r w rl wl rw)) ce cs ce'' cs''
-  .
+  (* Inductive eval_fstmt_single : hfstmt -> CE.env -> cstate -> CE.env -> cstate -> Prop := *)
+  (* | Eval_sskip : forall ce cs, eval_fstmt_single sskip ce cs ce cs *)
+  (* (* declare wire with ground type *) *)
+  (* | Eval_swire_gt v t ce cs ce' cs': *)
+  (*     CELemmas.P.Add v (t, Wire) ce ce' -> *)
+  (*     SV.Upd v (r_ftype (Gtyp t)) cs cs' -> *)
+  (*     eval_fstmt_single (swire v (Gtyp t)) ce cs ce' cs' *)
+  (* (* declare wire with vector type *) *)
+  (* | Eval_swire_agt v t n ce cs ce' cs' ce'' cs'': *)
+  (*     0 < n -> *)
+  (*     eval_fstmt_single (swire (new_vecvar v n) t) ce cs ce' cs' -> *)
+  (*     eval_fstmt_single (swire v (Atyp t n.-1)) ce' cs' ce'' cs'' -> *)
+  (*     eval_fstmt_single (swire v (Atyp t n)) ce cs ce'' cs'' *)
+  (* (* TBD. declare wire with bundle type *) *)
+  (* (*| Eval_swire_bt *) *)
+  (* (* declare node with expr, valid rhs *) *)
+  (* | Eval_snode v e ce cs ce' cs': *)
+  (*     valid_rhs_fexpr e ce' -> *)
+  (*     CELemmas.P.Add v ((type_of_hfexpr e ce), Node) ce ce' -> *)
+  (*     SV.Upd v (r_fexpr e) cs cs' -> *)
+  (*     eval_fstmt_single (snode v e) ce cs ce' cs' *)
+  (* (* define full connection *) *)
+  (* (* valid flow orient, type eq between dst and src, dst width upd to max (current size, src) *) *)
+  (* | Eval_sfcnct v e ce ce' cs cs': *)
+  (*     valid_lhs_orient (orient_of_comp (snd (CE.vtyp v ce))) -> *)
+  (*     valid_rhs_fexpr e ce -> *)
+  (*     fgtyp_equiv (fst (CE.vtyp v ce)) (type_of_hfexpr e ce) -> *)
+  (*     CELemmas.P.Add v (change_width (fst (CE.vtyp v ce)) (maxn (sizeof_fgtyp (fst (CE.vtyp v ce))) (sizeof_fgtyp (type_of_hfexpr e ce))), snd (CE.vtyp v ce)) ce ce' -> *)
+  (*     SV.Upd v (r_fexpr e) cs cs' -> *)
+  (*     eval_fstmt_single (sfcnct (Eref v) e) ce cs ce' cs' *)
+  (* (* declare reg with ground type , reset expr type equiv with reg type*) *)
+  (* | Eval_sreg_r_gt r t c rc rs ce cs ce' cs' : *)
+  (*     fgtyp_equiv (type_of_hfexpr rs ce) t -> *)
+  (*     CELemmas.P.Add r (t , Register) ce ce' -> *)
+  (*     SV.Upd r (r_fstmt (sreg (mk_hfreg r (Gtyp t) c (rrst rc rs)))) cs cs' -> *)
+  (*     eval_fstmt_single (sreg (mk_hfreg r (Gtyp t) c (rrst rc rs))) ce cs ce' cs' *)
+  (* (* declare reg with ground type, non reset *) *)
+  (* | Eval_sreg_nr_gt r t c ce cs ce' cs' : *)
+  (*     CELemmas.P.Add r (t , Register) ce ce' -> *)
+  (*     SV.Upd r (r_fstmt (sreg (mk_hfreg r (Gtyp t) c nrst))) cs cs' -> *)
+  (*     eval_fstmt_single (sreg (mk_hfreg r (Gtyp t) c nrst)) ce cs ce' cs' *)
+  (* (* declare reg with vector ground type *) *)
+  (* | Eval_sreg_agt r t n c rs ce cs ce' cs' ce'' cs'' : *)
+  (*     0 < n -> *)
+  (*     eval_fstmt_single (sreg (mk_hfreg r t c rs)) ce cs ce' cs' -> *)
+  (*     eval_fstmt_single (sreg (mk_hfreg r (Atyp t n.-1) c rs)) ce' cs' ce'' cs'' -> *)
+  (*     eval_fstmt_single (sreg (mk_hfreg r (Atyp t n) c rs)) ce cs ce'' cs'' *)
+  (* (* declare mem with ground type *) *)
+  (* | Eval_smem_gt m t dp r w rl wl rw ce cs ce' cs' : *)
+  (*     is_passive (Gtyp t) -> *)
+  (*     CELemmas.P.Add m (t, Memory) ce ce' -> *)
+  (*     SV.Upd m (r_fstmt (smem (mk_hfmem m (Gtyp t) dp r w rl wl rw))) cs cs' -> *)
+  (*     eval_fstmt_single (smem (mk_hfmem m (Gtyp t) dp r w rl wl rw)) ce cs ce' cs' *)
+  (* (* declare mem with vector ground type *) *)
+  (* | Eval_smem_agt m t n dp r w rl wl rw ce cs ce' cs' ce'' cs'': *)
+  (*     0 < n -> *)
+  (*     is_passive (Atyp (Gtyp t) n) -> *)
+  (*     CELemmas.P.Add m (t, Memory) ce ce' -> *)
+  (*     SV.Upd (new_vecvar m n) (r_fstmt (smem (mk_hfmem m (Gtyp t) dp r w rl wl rw))) cs cs' -> *)
+  (*     eval_fstmt_single (smem (mk_hfmem m (Atyp (Gtyp t) n.-1) dp r w rl wl rw)) ce' cs' ce'' cs'' -> *)
+  (*     eval_fstmt_single (smem (mk_hfmem m (Atyp (Gtyp t) n) dp r w rl wl rw)) ce cs ce'' cs'' *)
+  (* . *)
 
-  (** semantics of statement group, last cnct considered *)
-  Inductive eval_fstmts_group : seq hfstmt -> CE.env -> cstate -> CE.env -> cstate -> Prop :=
-  | Gnil ce cs: eval_fstmts_group [::] ce cs ce cs
-  (** connect to a dst *)
-  | Gfstmts_last_cncts v e hst_tl ce ce' cs cs' cs'' :
-      eval_fstmt_single (sfcnct (Eref v) e) ce cs ce cs' ->
-      eval_fstmts_group hst_tl ce cs' ce' cs'' ->
-      eval_fstmts_group (sfcnct (Eref v) e :: hst_tl) ce cs ce' cs''
-  (**  claim a sreg *)
-  | Gfstmts_reg_init (r: hfreg) hst_tl ce ce' ce'' cs cs' cs'' :
-      eval_fstmt_single (sreg r) ce cs ce' cs' ->
-      eval_fstmts_group  hst_tl ce' cs' ce'' cs'' ->
-      eval_fstmts_group (sreg r :: hst_tl) ce cs ce'' cs''
-  (** claim a node *)
-  | Gfstmts_node v e hst_tl ce ce' ce'' cs cs' cs'' :
-      eval_fstmt_single (snode v e) ce cs ce' cs' ->
-      eval_fstmts_group hst_tl ce' cs' ce'' cs'' ->
-      eval_fstmts_group (snode v e :: hst_tl) ce cs ce'' cs''
-  (** skip *)
-  | Gskip_fstmts hst_tl ce ce' cs cs' :
-      eval_fstmts_group hst_tl ce cs ce' cs' ->
-      eval_fstmts_group (sskip :: hst_tl) ce cs ce' cs'
-  (** condition when *)
-  | Gwhen_fstmts c hstg1 hstg2 hst_tl ce ce' ce'' cs cs' cs'' :
-      eval_fstmts_group_branch c hstg1 hstg2 ce cs ce' cs' ->
-      eval_fstmts_group hst_tl ce' cs' ce'' cs'' ->
-      eval_fstmts_group (swhen c hstg1 hstg2 :: hst_tl) ce cs ce'' cs''
-  (** https://github.com/llvm/circt/blob/main/lib/Dialect/FIRRTL/Transforms/ExpandWhens.cpp *)
-  with eval_fstmts_group_branch :
-         hfexpr -> seq hfstmt -> seq hfstmt -> CE.env -> cstate -> CE.env -> cstate -> Prop :=
-  (** nil *)
-  | Gthen_else_def c ce cs :
-      eval_fstmts_group_branch c [::] [::] ce cs ce cs 
-  (** connect to dst in then branch which has "not" been connected previously, add then branch *)
-  | Gthen_cnct_0 c v e hstg1 hstg2 ce ce' ce'' cs cs' cs'' :
-      CE.find v ce == None ->
-      eval_fstmt_single (sfcnct (eref v) e) ce cs ce' cs' ->
-      eval_fstmts_group_branch c hstg1 hstg2 ce' cs' ce'' cs'' ->
-      eval_fstmts_group_branch c (sfcnct (eref v) e :: hstg1) hstg2 ce cs ce'' cs''
-  (** connect to dst in else branch which has "not" been connected previously, add else branch *)
-  | Gelse_cnct_0 c v e hstg2 ce ce' ce'' cs cs' cs'' :
-      CE.find v ce == None ->
-      eval_fstmt_single (sfcnct (eref v) e) ce cs ce' cs' ->
-      eval_fstmts_group_branch c [::] hstg2 ce' cs' ce'' cs'' ->
-      eval_fstmts_group_branch c [::] (sfcnct (eref v) e :: hstg2) ce cs ce'' cs''
-  (** connect to dst in then branch which has been connected previously, add mux(p, then, prev) *)
-  | Gthen_cnct c v e re hstg1 hstg2 ce ce' cs cs' cs'' :
-      SV.acc v cs == r_fexpr re ->
-      (* CELemmas.P.Add vn Node ce ce' -> *)
-      (* SV.Upd vn (r_fexpr (emux c e re)) cs cs' -> *)
-      SV.Upd v (r_fexpr (emux c e re)) cs cs' ->
-      eval_fstmts_group_branch c hstg1 hstg2 ce cs' ce' cs'' ->
-      eval_fstmts_group_branch c (sfcnct (eref v) e :: hstg1) hstg2 ce cs ce' cs''
-  (** connect to dst in else branch which has been connected previously, add mux(p, prev, else) *)
-  | Gelse_cnct c v e re hstg2 ce ce' cs cs' cs'' :
-      SV.acc v cs == r_fexpr re ->
-      SV.Upd v (r_fexpr (emux c re e)) cs cs' ->
-      eval_fstmts_group_branch c [::] hstg2 ce cs' ce' cs'' ->
-      eval_fstmts_group_branch c [::] (sfcnct (eref v) e :: hstg2) ce cs ce' cs''
-  (** claim a sreg in then branch *)
-  | Gthen_reg c r hstg1 hstg2 ce ce' ce'' cs cs' cs'' :
-      eval_fstmt_single (sreg r) ce cs ce' cs' ->
-      eval_fstmts_group_branch c hstg1 hstg2 ce' cs' ce'' cs'' ->
-      eval_fstmts_group_branch c (sreg r :: hstg1) hstg2 ce cs ce'' cs''
-  (** claim a sreg in else branch *)
-  | Gelse_reg c r hstg2 ce ce' ce'' cs cs' cs'' :
-      eval_fstmt_single (sreg r) ce cs ce' cs' ->
-      eval_fstmts_group_branch c [::] hstg2 ce' cs' ce'' cs'' ->
-      eval_fstmts_group_branch c [::] (sreg r :: hstg2) ce cs ce'' cs''
-  (** claim a node in then branch *)
-  | Gthen_node c v e hstg1 hstg2 ce ce' ce'' cs cs' cs'' :
-      eval_fstmt_single (snode v e) ce cs ce' cs' ->
-      eval_fstmts_group_branch c hstg1 hstg2 ce' cs' ce'' cs'' ->
-      eval_fstmts_group_branch c (snode v e :: hstg1) hstg2 ce cs ce'' cs''
-  (** claim a node in else branch *)
-  | Gelse_node c v e hstg2 ce ce' ce'' cs cs' cs'' :
-      eval_fstmt_single (snode v e) ce cs ce' cs' ->
-      eval_fstmts_group_branch c [::] hstg2 ce' cs' ce'' cs'' ->
-      eval_fstmts_group_branch c [::] (snode v e :: hstg2) ce cs ce'' cs''
-  .
+  (* (** semantics of statement group, last cnct considered *) *)
+  (* Inductive eval_fstmts_group : seq hfstmt -> CE.env -> cstate -> CE.env -> cstate -> Prop := *)
+  (* | Gnil ce cs: eval_fstmts_group [::] ce cs ce cs *)
+  (* (** connect to a dst *) *)
+  (* | Gfstmts_last_cncts v e hst_tl ce ce' cs cs' cs'' : *)
+  (*     eval_fstmt_single (sfcnct (Eref v) e) ce cs ce cs' -> *)
+  (*     eval_fstmts_group hst_tl ce cs' ce' cs'' -> *)
+  (*     eval_fstmts_group (sfcnct (Eref v) e :: hst_tl) ce cs ce' cs'' *)
+  (* (**  claim a sreg *) *)
+  (* | Gfstmts_reg_init (r: hfreg) hst_tl ce ce' ce'' cs cs' cs'' : *)
+  (*     eval_fstmt_single (sreg r) ce cs ce' cs' -> *)
+  (*     eval_fstmts_group  hst_tl ce' cs' ce'' cs'' -> *)
+  (*     eval_fstmts_group (sreg r :: hst_tl) ce cs ce'' cs'' *)
+  (* (** claim a node *) *)
+  (* | Gfstmts_node v e hst_tl ce ce' ce'' cs cs' cs'' : *)
+  (*     eval_fstmt_single (snode v e) ce cs ce' cs' -> *)
+  (*     eval_fstmts_group hst_tl ce' cs' ce'' cs'' -> *)
+  (*     eval_fstmts_group (snode v e :: hst_tl) ce cs ce'' cs'' *)
+  (* (** skip *) *)
+  (* | Gskip_fstmts hst_tl ce ce' cs cs' : *)
+  (*     eval_fstmts_group hst_tl ce cs ce' cs' -> *)
+  (*     eval_fstmts_group (sskip :: hst_tl) ce cs ce' cs' *)
+  (* (** condition when *) *)
+  (* | Gwhen_fstmts c hstg1 hstg2 hst_tl ce ce' ce'' cs cs' cs'' : *)
+  (*     eval_fstmts_group_branch c hstg1 hstg2 ce cs ce' cs' -> *)
+  (*     eval_fstmts_group hst_tl ce' cs' ce'' cs'' -> *)
+  (*     eval_fstmts_group (swhen c hstg1 hstg2 :: hst_tl) ce cs ce'' cs'' *)
+  (* (** https://github.com/llvm/circt/blob/main/lib/Dialect/FIRRTL/Transforms/ExpandWhens.cpp *) *)
+  (* with eval_fstmts_group_branch : *)
+  (*        hfexpr -> seq hfstmt -> seq hfstmt -> CE.env -> cstate -> CE.env -> cstate -> Prop := *)
+  (* (** nil *) *)
+  (* | Gthen_else_def c ce cs : *)
+  (*     eval_fstmts_group_branch c [::] [::] ce cs ce cs  *)
+  (* (** connect to dst in then branch which has "not" been connected previously, add then branch *) *)
+  (* | Gthen_cnct_0 c v e hstg1 hstg2 ce ce' ce'' cs cs' cs'' : *)
+  (*     CE.find v ce == None -> *)
+  (*     eval_fstmt_single (sfcnct (eref v) e) ce cs ce' cs' -> *)
+  (*     eval_fstmts_group_branch c hstg1 hstg2 ce' cs' ce'' cs'' -> *)
+  (*     eval_fstmts_group_branch c (sfcnct (eref v) e :: hstg1) hstg2 ce cs ce'' cs'' *)
+  (* (** connect to dst in else branch which has "not" been connected previously, add else branch *) *)
+  (* | Gelse_cnct_0 c v e hstg2 ce ce' ce'' cs cs' cs'' : *)
+  (*     CE.find v ce == None -> *)
+  (*     eval_fstmt_single (sfcnct (eref v) e) ce cs ce' cs' -> *)
+  (*     eval_fstmts_group_branch c [::] hstg2 ce' cs' ce'' cs'' -> *)
+  (*     eval_fstmts_group_branch c [::] (sfcnct (eref v) e :: hstg2) ce cs ce'' cs'' *)
+  (* (** connect to dst in then branch which has been connected previously, add mux(p, then, prev) *) *)
+  (* | Gthen_cnct c v e re hstg1 hstg2 ce ce' cs cs' cs'' : *)
+  (*     SV.acc v cs == r_fexpr re -> *)
+  (*     (* CELemmas.P.Add vn Node ce ce' -> *) *)
+  (*     (* SV.Upd vn (r_fexpr (emux c e re)) cs cs' -> *) *)
+  (*     SV.Upd v (r_fexpr (emux c e re)) cs cs' -> *)
+  (*     eval_fstmts_group_branch c hstg1 hstg2 ce cs' ce' cs'' -> *)
+  (*     eval_fstmts_group_branch c (sfcnct (eref v) e :: hstg1) hstg2 ce cs ce' cs'' *)
+  (* (** connect to dst in else branch which has been connected previously, add mux(p, prev, else) *) *)
+  (* | Gelse_cnct c v e re hstg2 ce ce' cs cs' cs'' : *)
+  (*     SV.acc v cs == r_fexpr re -> *)
+  (*     SV.Upd v (r_fexpr (emux c re e)) cs cs' -> *)
+  (*     eval_fstmts_group_branch c [::] hstg2 ce cs' ce' cs'' -> *)
+  (*     eval_fstmts_group_branch c [::] (sfcnct (eref v) e :: hstg2) ce cs ce' cs'' *)
+  (* (** claim a sreg in then branch *) *)
+  (* | Gthen_reg c r hstg1 hstg2 ce ce' ce'' cs cs' cs'' : *)
+  (*     eval_fstmt_single (sreg r) ce cs ce' cs' -> *)
+  (*     eval_fstmts_group_branch c hstg1 hstg2 ce' cs' ce'' cs'' -> *)
+  (*     eval_fstmts_group_branch c (sreg r :: hstg1) hstg2 ce cs ce'' cs'' *)
+  (* (** claim a sreg in else branch *) *)
+  (* | Gelse_reg c r hstg2 ce ce' ce'' cs cs' cs'' : *)
+  (*     eval_fstmt_single (sreg r) ce cs ce' cs' -> *)
+  (*     eval_fstmts_group_branch c [::] hstg2 ce' cs' ce'' cs'' -> *)
+  (*     eval_fstmts_group_branch c [::] (sreg r :: hstg2) ce cs ce'' cs'' *)
+  (* (** claim a node in then branch *) *)
+  (* | Gthen_node c v e hstg1 hstg2 ce ce' ce'' cs cs' cs'' : *)
+  (*     eval_fstmt_single (snode v e) ce cs ce' cs' -> *)
+  (*     eval_fstmts_group_branch c hstg1 hstg2 ce' cs' ce'' cs'' -> *)
+  (*     eval_fstmts_group_branch c (snode v e :: hstg1) hstg2 ce cs ce'' cs'' *)
+  (* (** claim a node in else branch *) *)
+  (* | Gelse_node c v e hstg2 ce ce' ce'' cs cs' cs'' : *)
+  (*     eval_fstmt_single (snode v e) ce cs ce' cs' -> *)
+  (*     eval_fstmts_group_branch c [::] hstg2 ce' cs' ce'' cs'' -> *)
+  (*     eval_fstmts_group_branch c [::] (snode v e :: hstg2) ce cs ce'' cs'' *)
+  (* . *)
 
   (* Lemma valid_conncection v e2 sts ce cs ce' cs' : *)
   (*   eval_fstmts_group (sfcnct (eref v) e2 :: sts) ce cs ce' cs' -> *)
